

Free types and induction

$[N]$

$Tree ::= stalk \mid leaf \langle\langle N \rangle\rangle \mid branch \langle\langle Tree \times Tree \rangle\rangle$

Solution 44

The two cases of the proof are established by equational reasoning: the first by

$$\text{reverse } (\langle \rangle^t) = \text{reverset}[cat.1a] = (\text{reverset})\langle \rangle \text{ [cat.1b]}$$

where $cat.1a$ is $\langle \rangle s = sandcat.1biss \langle \rangle = s$

and the second by

$$\text{reverse } ((\langle x \rangle^u)^t) = \text{reverse}(\langle x \rangle^{\langle u^t \rangle})[cat.2]$$

$$= \text{reverse } (u^t \langle x \rangle) [\text{reverse.2}]$$

$$= (\text{reverse } t^{\text{reverse} u}) \langle x \rangle \text{ [anti-distributive]}$$

$$= \text{reverse } t^{\langle \text{reverse} u \rangle} \langle x \rangle \text{ [cat.2]}$$

$$= \text{reverse } t^{\text{reverse} \langle x \rangle^u} [\text{reverse.2}]$$

Solution 45

The base case:

$$\text{reverse} (\text{reverse } \langle \rangle) = \text{reverse } \langle \rangle [\text{reverse.1}] = \langle \rangle [\text{reverse.1}]$$

The inductive step:

$$\begin{aligned} & \text{reverse} (\text{reverse } (\langle x \rangle^t)) \\ &= \text{reverse} ((\text{reverse } t) \langle x \rangle) [\text{reverse.2}] \\ &= \text{reverse} (\langle x \rangle) {}^r\text{everse}(\text{reverset})[\text{anti} - \text{distributive}] \\ &= \text{reverse} (\langle x \rangle \langle \rangle) {}^r\text{everse}(\text{reverset})[\text{cat.1}] \\ &= ((\text{reverse } \langle \rangle) \langle x \rangle) {}^r\text{everse}(\text{reverset})[\text{reverse.2}] \\ &= (\langle \rangle \langle x \rangle) {}^r\text{everse}(\text{reverset})[\text{reverse.1}] \\ &= \langle x \rangle {}^r\text{everse}(\text{reverset})[\text{cat.1}] \\ &= \langle x \rangle^t [\text{reverse}(\text{reverset}) = t] \end{aligned}$$

Solution 46

(a)

$$\text{count} : \text{Tree} \rightarrow N$$

$$\text{count } \text{stalk} = 0$$

$$\forall n: N \bullet \text{count}(\text{leaf } n) = 1$$

$$\forall t1, t2: Tree \bullet \text{count}(\text{branch}(t1, t2)) = \text{count } t1 + \text{count } t2$$

(Blocked by: recursive free types and pattern matching)

(b)

$$\text{flatten} : Tree \rightarrow seq\ N$$

$$\text{flatten stalk} = \langle \rangle$$

$$\forall n: N \bullet \text{flatten}(\text{leaf } n) = \langle n \rangle$$

$$\forall t1, t2: Tree \bullet \text{flatten}(\text{branch}(t1, t2)) = \text{flatten } t1 \ ^f \text{flatten } t2$$

(Blocked by: recursive free types and pattern matching)

Solution 47

First, exhibit the induction principle for the free type:

$$P \text{ stalk and } (\forall n: N \bullet P(\text{leaf } n)) \text{ and } (\forall t1, t2: Tree \bullet P\ t1 \wedge P\ t2 \Rightarrow P\ \text{branch}(t1, t2))$$

$$\text{implies } \forall t: Tree \bullet P\ t$$

This gives three cases for the proof:

$$(\text{flatten stalk}) = \langle \rangle \ [\text{flatten}] = 0 \ [] = \text{count stalk} \ [\text{count}]$$

(Remaining cases omitted - require equational reasoning with recursive functions)